Formalise matcher without inhab

RegexPosix/POSIX.lean
@@ -31,6 +31,30 @@ inductive POSIX : Regex α → Value α → Prop
     ¬(∃ s₃ s₄, s₃ ≠ [] ∧ s₃ ++ s₄ = (stars vs).flat ∧ r.Matches (v.flat ++ s₃) ∧ (star r).Matches s₄) →
     POSIX (star r) (stars (v::vs))
 
+inductive POSIX' : {r : Regex α} → Parse r → Prop
+  | epsilon : POSIX' Parse.empty
+  | char (c : α) : POSIX' (Parse.char c)
+  | left {r₁ : Regex α} {p : Parse r₁} :
+    POSIX' p →
+    POSIX' p.left
+  | right {r₁ r₂ : Regex α} {p : Parse r₂} :
+    POSIX' p →
+    ¬r₁.Matches p.flat →
+    @POSIX' (r₁.plus r₂) p.right
+  | mul {r₁ r₂ : Regex α} {p₁ : Parse r₁} {p₂ : Parse r₂} :
+    POSIX' p₁ →
+    POSIX' p₂ →
+    ¬(∃ s₃ s₄, s₃ ≠ [] ∧ s₃ ++ s₄ = p₂.flat ∧ r₁.Matches (p₁.flat ++ s₃) ∧ r₂.Matches s₄) →
+    POSIX' (p₁.seq p₂)
+  | star_nil :
+    POSIX' Parse.star_nil
+  | stars {r : Regex α} {p : Parse r} {ps : Parse (star r)} :
+    POSIX' p →
+    POSIX' ps →
+    p.flat ≠ [] →
+    ¬(∃ s₃ s₄, s₃ ≠ [] ∧ s₃ ++ s₄ = ps.flat ∧ r.Matches (p.flat ++ s₃) ∧ (star r).Matches s₄) →
+    POSIX' (p.star_cons ps)
+
 theorem POSIX.inhab {r : Regex α} {v : Value α} : POSIX r v → Inhab v r
   | epsilon => Inhab.empty
   | char c => Inhab.char c
@@ -42,6 +66,9 @@ theorem POSIX.inhab {r : Regex α} {v : Value α} : POSIX r v → Inhab v r
 
 theorem POSIX.matches {r : Regex α} {v : Value α} : POSIX r v → r.Matches v.flat :=
   fun h => h.inhab.matches
+
+theorem POSIX'.matches {r : Regex α} {p : Parse r} : POSIX' p → r.Matches p.flat :=
+  fun _ => p.matches
 
 theorem longest_split_unique {r₁ r₂ : Regex α} {s₁₁ s₁₂ s₂₁ s₂₂ : List α}
   (hs : s₁₁ ++ s₁₂ = s₂₁ ++ s₂₂)
@@ -66,6 +93,59 @@ theorem longest_split_unique {r₁ r₂ : Regex α} {s₁₁ s₁₂ s₂₁ s�
     | nil => rfl
     | cons x xs =>
       exact absurd hr₁₂ (h₂ (x::xs) (by simp) s₁₂ rfl hr₁₁)
+
+theorem POSIX'.unique {r : Regex α} {p₁ p₂ : Parse r} (hp : p₁.flat = p₂.flat) (h₁ : POSIX' p₁) (h₂ : POSIX' p₂) :
+  p₁ = p₂ := by
+  induction h₁ with
+  | epsilon =>
+    cases h₂
+    rfl
+  | char c =>
+    cases h₂
+    rfl
+  | left h₁ ih =>
+    cases h₂ with
+    | left h₂ =>
+      rw [Parse.left.injEq]
+      simp at hp
+      exact ih hp h₂
+    | right h₂ hn =>
+      simp at hp
+      rw [←hp] at hn
+      exact absurd h₁.matches hn
+  | right h₁ hn ih =>
+    cases h₂ with
+    | left h₂ =>
+      simp at hp
+      rw [hp] at hn
+      exact absurd h₂.matches hn
+    | right h₂ hn' =>
+      rw [Parse.right.injEq]
+      simp at hp
+      exact ih hp h₂
+  | mul h₁₁ h₁₂ hs₁ ih₁ ih₂ =>
+    cases h₂ with
+    | mul h₂₁ h₂₂ hs₂ =>
+      simp at hp
+      have hv' := longest_split_unique hp h₁₁.matches h₁₂.matches h₂₁.matches h₂₂.matches hs₁ hs₂
+      rw [ih₁ hv'.left h₂₁, ih₂ hv'.right h₂₂]
+  | star_nil =>
+    cases h₂ with
+    | star_nil => rfl
+    | stars _ _ hp' =>
+      simp at hp
+      exact absurd hp.left hp'
+  | stars h₁₁ h₁₂ hp₁ hs₁ ih₁ ih₂ =>
+    cases h₂ with
+    | star_nil =>
+      simp at hp
+      exact absurd hp.left hp₁
+    | stars h₂₁ h₂₂ hp₂ hs₂ =>
+      simp at hp
+      have hv' := longest_split_unique hp h₁₁.matches h₁₂.matches h₂₁.matches h₂₂.matches hs₁ hs₂
+      have ih₂ := ih₂ hv'.right h₂₂
+      simp at ih₂
+      rw [ih₁ hv'.left h₂₁, ih₂]
 
 theorem POSIX.unique {r : Regex α} {v₁ v₂ : Value α} (hv : v₁.flat = v₂.flat) (h₁ : POSIX r v₁) (h₂ : POSIX r v₂) :
   v₁ = v₂ := by
