RegexPosix/Parse.lean
@@ -1,4 +1,5 @@
 import RegexPosix.Value
+import Mathlib.Tactic.GeneralizeProofs
 
 open Value
 open Regex
@@ -43,7 +44,52 @@ theorem mkeps_flat {α : Type u} {r : Regex α} (hn : r.nullable) :
     rw [ih₁, ih₂, and_self]
   | star r ih => simp [mkeps]
 
+def mkeps' : {r : Regex α} → r.nullable → Parse r
+  | epsilon, _ => Parse.empty
+  | plus r₁ _, hn =>
+    if hn₁ : r₁.nullable
+      then
+        Parse.left (mkeps' hn₁)
+      else
+        have hn₂ := (Bool.or_eq_true_iff.mp hn).resolve_left hn₁
+        Parse.right (mkeps' hn₂)
+  | mul _ _, hn =>
+    have ⟨hn₁, hn₂⟩ := Bool.and_eq_true_iff.mp hn
+    Parse.seq (mkeps' hn₁) (mkeps' hn₂)
+  | star _, _ => Parse.star_nil
+
+theorem mkeps'_flat {r : Regex α} {hn : r.nullable} :
+  (mkeps' hn).flat = [] := by
+  fun_induction mkeps' with
+  | case1 => rfl
+  | case2 r₁ r₂ hn hn₁ ih₁ =>
+    simp only [Parse.flat, ih₁]
+  | case3 r₁ r₂ hn hn₁ hn₂ ih₂ =>
+    simp only [Parse.flat, ih₂]
+  | case4 r₁ r₂ hn hn₁ hn₂ ih₁ ih₂ =>
+    simp [ih₁, ih₂]
+  | case5 => rfl
+
 variable [DecidableEq α]
+
+def inj' : {r : Regex α} → (c : α) → Parse (r.deriv c) → Parse r
+  | .char d, _c, _ => Parse.char d
+  | .plus r₁ r₂, c, Parse.left p => Parse.left (inj' c p)
+  | .plus r₁ r₂, c, Parse.right p => Parse.right (inj' c p)
+  | .mul r₁ _, c, p =>
+    if hn₁ : r₁.nullable
+      then
+        match (deriv_mul_nullable hn₁) ▸ p with
+        | Parse.left (Parse.seq p₁ p₂) =>
+          Parse.seq (inj' c p₁) p₂
+        | Parse.right p₂ =>
+          Parse.seq (mkeps' hn₁) (inj' c p₂)
+      else
+        match (deriv_mul_not_nullable hn₁) ▸ p with
+        | Parse.seq p₁ p₂ =>
+          Parse.seq (inj' c p₁) p₂
+  | .star r, c, Parse.seq p ps =>
+    Parse.star_cons (inj' c p) ps
 
 def inj : (r : Regex α) → (c : α) → (Σ' v : Value α, Inhab v (r.deriv c)) → (Σ' v : Value α, Inhab v r)
   | .char d, c, ⟨v, h⟩ => ⟨Value.char d, Inhab.char d⟩
@@ -71,6 +117,43 @@ def inj : (r : Regex α) → (c : α) → (Σ' v : Value α, Inhab v (r.deriv c)
   | .star r, c, ⟨Value.seq v (Value.stars vs), h⟩ =>
     have ⟨v, hv⟩ := inj r c ⟨v, inhab_seq_fst h⟩
     ⟨Value.stars (v :: vs), Inhab.stars hv (inhab_seq_snd h)⟩
+
+theorem inj'_flat {r : Regex α} {c : α} {p : Parse (r.deriv c)} :
+  (inj' c p).flat = c::p.flat := by
+  fun_induction inj' with
+  | case1 d c p =>
+    generalize hr : (Regex.char d).deriv c = r' at p
+    rw [Regex.deriv] at hr
+    split_ifs at hr with hc
+    · subst hr hc
+      cases p
+      simp only [Parse.flat]
+    · subst hr
+      nomatch p
+  | case2 r₁ r₂ c p ih =>
+    simp only [Parse.flat, ih]
+  | case3 r₁ r₂ c p ih =>
+    simp only [Parse.flat, ih]
+  | case4 r₁ r₂ c hn p₁ p₂ p heq ih₁ =>
+    generalize_proofs k at heq
+    generalize hr : (r₁.mul r₂).deriv c = r' at *
+    simp [deriv, hn] at hr
+    subst hr heq
+    simp [ih₁]
+  | case5 r₁ r₂ c hn p₂ p heq ih₂ =>
+    generalize_proofs k at heq
+    generalize hr : (r₁.mul r₂).deriv c = r' at *
+    simp [deriv, hn] at hr
+    subst hr heq
+    simp [mkeps'_flat, ih₂]
+  | case6 r₁ r₂ c hn p₁ p₂ p heq ih₁ =>
+    generalize_proofs k at heq
+    generalize hr : (r₁.mul r₂).deriv c = r' at *
+    simp [deriv, hn] at hr
+    subst hr heq
+    simp [ih₁]
+  | case7 r c p ps ih =>
+    simp [ih]
 
 theorem inj_flat {r : Regex α} {c : α} {v : Value α} (hv : Inhab v (r.deriv c)) :
   (inj r c ⟨v, hv⟩).fst.flat = c::v.flat := by
@@ -106,9 +189,21 @@ theorem inj_flat {r : Regex α} {c : α} {v : Value α} (hv : Inhab v (r.deriv c
     | Value.seq v (Value.stars vs) =>
       simp [inj, ih]
 
+def injs' : {r : Regex α} → (s : List α) → (Parse (r.derivs s)) → Parse r
+  | _, [], p => p
+  | _, c::s, p => inj' c (injs' s p)
+
 def injs : (r : Regex α) → (s : List α) → (Σ' v : Value α, Inhab v (r.derivs s)) → (Σ' v' : Value α, Inhab v' r)
   | _, [], h => h
   | r, c::s, h => inj r c (injs (r.deriv c) s h)
+
+theorem injs'_flat {r : Regex α} {s : List α} {p : Parse (r.derivs s)} :
+  (injs' s p).flat = s ++ p.flat := by
+  induction s generalizing r with
+  | nil => rfl
+  | cons x xs ih =>
+    simp [injs']
+    rw [inj'_flat, ih]
 
 theorem injs_flat {r : Regex α} {s : List α} {v : Value α} (hv : Inhab v (r.derivs s)) :
   (injs r s ⟨v, hv⟩).fst.flat = s ++ v.flat := by
@@ -117,6 +212,13 @@ theorem injs_flat {r : Regex α} {s : List α} {v : Value α} (hv : Inhab v (r.d
   | cons x xs ih =>
     simp [injs]
     rw [inj_flat, ih hv]
+
+def Regex.parse' : (r : Regex α) → List α → Option (Parse r)
+  | r, s =>
+    let r' := r.derivs s
+    if h : r'.nullable
+      then some (injs' s (mkeps' h))
+      else none
 
 def Regex.parse : Regex α → List α → Option (Value α)
   | r, s =>
@@ -131,6 +233,14 @@ theorem parse_flat {r : Regex α} {s : List α} {v : Value α} :
   simp [parse] at h
   rcases h with ⟨hn, h⟩
   rw [←h, injs_flat, mkeps_flat]
+  exact List.append_nil s
+
+theorem parse'_flat {r : Regex α} {s : List α} {p : Parse r} :
+  r.parse' s = some p → p.flat = s := by
+  intro h
+  simp [parse'] at h
+  rcases h with ⟨hn, h⟩
+  rw [←h, injs'_flat, mkeps'_flat]
   exact List.append_nil s
 
 theorem parse_matches_iff {r : Regex α} (s : List α) :
