RegexPosix/Value.lean
@@ -28,6 +28,62 @@ def Value.flat : Value α → List α
 open Value
 open Regex
 
+inductive Parse : Regex α → Type u
+  | empty : Parse epsilon
+  | char (c : α) : Parse (char c)
+  | left {r₁ r₂ : Regex α} :
+    Parse r₁ →
+    Parse (r₁.plus r₂)
+  | right {r₁ r₂ : Regex α} :
+    Parse r₂ →
+    Parse (r₁.plus r₂)
+  | seq {r₁ r₂ : Regex α} :
+    Parse r₁ →
+    Parse r₂ →
+    Parse (r₁.mul r₂)
+  | star_nil {r : Regex α} :
+    Parse r.star
+  | star_cons {r : Regex α} :
+    Parse r →
+    Parse r.star →
+    Parse r.star
+
+protected def Parse.repr [Repr α] {r : Regex α} (p : Parse r) (n : Nat) : Std.Format :=
+  let _ : Std.ToFormat α := ⟨repr⟩
+  match r, n with
+  | Regex.epsilon, _ => "Empty"
+  | Regex.char c, _ => "Char " ++ repr c
+  | Regex.plus _ _, n =>
+    match p with
+    | Parse.left p => "Left (" ++ p.repr n ++ ")"
+    | Parse.right p => "Right (" ++ p.repr n ++ ")"
+  | Regex.mul _ _, n =>
+    match p with
+    | Parse.seq p₁ p₂ => "Seq (" ++ p₁.repr n ++ ") (" ++ p₂.repr n ++ ")"
+  | Regex.star r, _ =>
+    match p with
+    | star_nil => "Stars []"
+    | ps => "Stars [" ++ reprStars ps n ++ "]"
+    where
+      reprStars [Repr α] {r : Regex α} (p : Parse (star r)) (n : Nat) : Std.Format :=
+        match p, n with
+        | Parse.star_nil, _ => ""
+        | Parse.star_cons p Parse.star_nil, n => p.repr n
+        | Parse.star_cons p ps, n => p.repr n ++ ", " ++ reprStars ps n
+
+instance [Repr α] {r : Regex α} : Repr (Parse r) where
+  reprPrec := Parse.repr
+
+@[simp]
+def Parse.flat {r : Regex α} : Parse r → List α
+  | empty => []
+  | char c => [c]
+  | left p => p.flat
+  | right p => p.flat
+  | seq p₁ p₂ => p₁.flat ++ p₂.flat
+  | star_nil => []
+  | star_cons p ps => p.flat ++ ps.flat
+
 inductive Inhab : Value α → Regex α → Prop
   | empty : Inhab empty epsilon
   | char (c : α) : Inhab (char c) (char c)
@@ -57,6 +113,16 @@ theorem Inhab.matches {r : Regex α} {v : Value α} :
   | seq h₁ h₂ => (Value.flat.eq_def _) ▸ Matches.mul rfl h₁.matches h₂.matches
   | star_nil => (Value.flat.eq_def _) ▸ Matches.star_nil
   | stars h₁ h₂ => (Value.flat.eq_def _) ▸ Matches.stars rfl h₁.matches h₂.matches
+
+theorem Parse.matches {r : Regex α} :
+  (p : Parse r) → r.Matches p.flat
+  | empty => Matches.epsilon
+  | char c => Matches.char
+  | left p => p.matches.left
+  | right p => p.matches.right
+  | seq p₁ p₂ => Matches.mul rfl p₁.matches p₂.matches
+  | star_nil => Matches.star_nil
+  | star_cons p ps => Matches.stars rfl p.matches ps.matches
 
 theorem matches_inhab {r : Regex α} {s : List α} :
   r.Matches s → ∃ v, v.flat = s ∧ Inhab v r := by
