RegexPosix/Correctness.lean
@@ -8,6 +8,21 @@ universe u
 
 variable {α : Type u}
 
+theorem mkeps'_posix {r : Regex α} {hn : r.nullable} :
+  POSIX' (mkeps' hn) := by
+  fun_induction mkeps' with
+  | case1 => exact POSIX'.epsilon
+  | case2 r₁ r₂ hn hn₁ ih₁ =>
+    exact POSIX'.left ih₁
+  | case3 r₁ r₂ hn hn₁ hn₂ ih₂ =>
+    refine POSIX'.right ih₂ ?_
+    rw [mkeps'_flat]
+    rw [←nullable_iff_matches_nil]
+    exact hn₁
+  | case4 r₁ r₂ hn hn₁ hn₂ ih₁ ih₂ =>
+    exact POSIX'.mul ih₁ ih₂ (by simp [mkeps'_flat])
+  | case5 r hn => exact POSIX'.star_nil
+
 theorem mkeps_posix {r : Regex α} (hn : r.nullable) :
   POSIX r (r.mkeps hn).fst := by
   induction r with
@@ -36,6 +51,66 @@ theorem mkeps_posix {r : Regex α} (hn : r.nullable) :
     apply POSIX.star_nil
 
 variable [DecidableEq α]
+
+theorem inj'_posix {r : Regex α} {c : α} {p : Parse (r.deriv c)} (h : POSIX' p) :
+  POSIX' (inj' c p) := by
+  fun_induction inj' with
+  | case1 d c p =>
+    exact POSIX'.char d
+  | case2 r₁ r₂ c p ih₁ =>
+    cases h with
+    | left h =>
+      exact POSIX'.left (ih₁ h)
+  | case3 r₁ r₂ c p ih₂ =>
+    cases h with
+    | right h hn =>
+      refine POSIX'.right (ih₂ h) ?_
+      rw [inj'_flat, Matches.deriv_iff]
+      exact hn
+  | case4 r₁ r₂ c hn₁ p₁ p₂ p heq ih₁ =>
+    generalize_proofs k at heq
+    generalize hr : (r₁.mul r₂).deriv c = r' at *
+    simp [hn₁] at hr
+    subst hr heq
+    cases h with
+    | left h =>
+      cases h with
+      | mul h₁ h₂ hs =>
+        refine POSIX'.mul (ih₁ h₁) h₂ ?_
+        simp_rw [inj'_flat, List.cons_append, Matches.deriv_iff]
+        exact hs
+  | case5 r₁ r₂ c hn₁ p₂ p heq ih₂ =>
+    generalize_proofs k at heq
+    generalize hr : (r₁.mul r₂).deriv c = r' at *
+    simp [hn₁] at hr
+    subst hr heq
+    cases h with
+    | right h hn =>
+      refine POSIX'.mul (mkeps'_posix) (ih₂ h) ?_
+      simp [inj'_flat, mkeps'_flat]
+      intro x hx y hxy hr₁ hr₂
+      rw [List.append_eq_cons_iff] at hxy
+      simp [hx] at hxy
+      rcases hxy with ⟨z, hx, hs⟩
+      rw [hx, Matches.deriv_iff] at hr₁
+      rw [hs] at hn
+      exact absurd (Matches.mul rfl hr₁ hr₂) hn
+  | case6 r₁ r₂ c hn₁ p₁ p₂ p heq ih₁ =>
+    generalize_proofs k at heq
+    generalize hr : (r₁.mul r₂).deriv c = r' at *
+    simp [hn₁] at hr
+    subst hr heq
+    cases h with
+    | mul h₁ h₂ hs =>
+      refine POSIX'.mul (ih₁ h₁) h₂ ?_
+      simp_rw [inj'_flat, List.cons_append, Matches.deriv_iff]
+      exact hs
+  | case7 r c p ps ih =>
+    cases h with
+    | mul h₁ h₂ hs =>
+      refine POSIX'.stars (ih h₁) h₂ (by simp [inj'_flat]) ?_
+      simp_rw [inj'_flat, List.cons_append, Matches.deriv_iff]
+      exact hs
 
 theorem inj_posix {r : Regex α} {v : Value α} {c : α} (h : POSIX (r.deriv c) v) :
   POSIX r (inj r c ⟨v, h.inhab⟩).fst := by
@@ -109,6 +184,15 @@ theorem inj_posix {r : Regex α} {v : Value α} {c : α} (h : POSIX (r.deriv c) 
         simp_rw [inj_flat, List.cons_append, Matches.deriv_iff]
         exact hs
 
+theorem injs'_posix {r : Regex α} {s : List α} {p : Parse (r.derivs s)} (h : POSIX' p) :
+  POSIX' (injs' s p) := by
+  induction s generalizing r with
+  | nil =>
+    exact h
+  | cons x xs ih =>
+    rw [injs']
+    exact inj'_posix (ih h)
+
 theorem injs_posix {r : Regex α} {v : Value α} {s : List α} (h : POSIX (r.derivs s) v) :
   POSIX r (injs r s ⟨v, h.inhab⟩).fst := by
   induction s generalizing r with
@@ -120,6 +204,16 @@ theorem injs_posix {r : Regex α} {v : Value α} {s : List α} (h : POSIX (r.der
     simp [injs]
     apply inj_posix
     exact ih h
+
+theorem matches_parse'_posix_iff {r : Regex α} {s : List α} :
+  r.Matches s ↔ ∃ p, r.parse' s = some p ∧ POSIX' p := by
+  simp [parse']
+  rw [Matches.derivs_iff, ←nullable_iff_matches_nil]
+  constructor
+  · intro h
+    exact ⟨h, injs'_posix mkeps'_posix⟩
+  · intro ⟨h, _⟩
+    exact h
 
 theorem matches_parse_posix_iff {r : Regex α} {s : List α} :
   r.Matches s ↔ ∃ v, r.parse s = some v ∧ POSIX r v := by
@@ -144,4 +238,19 @@ theorem parse_posix_iff (r : Regex α) (s : List α) (v : Value α) :
     subst hv
     rcases (matches_parse_posix_iff.mp h.matches) with ⟨v', h', h''⟩
     rw [POSIX.unique (parse_flat h') h'' h] at h'
+    exact h'
+
+theorem parse'_posix_iff (r : Regex α) (s : List α) (p : Parse r) :
+  r.parse' s = some p ↔ p.flat = s ∧ POSIX' p := by
+  constructor
+  · intro h
+    refine ⟨parse'_flat h, ?_⟩
+    simp [parse'] at h
+    rcases h with ⟨hn, h⟩
+    rw [←h]
+    exact injs'_posix mkeps'_posix
+  · intro ⟨hv, h⟩
+    subst hv
+    rcases (matches_parse'_posix_iff.mp h.matches) with ⟨v', h', h''⟩
+    rw [POSIX'.unique (parse'_flat h') h'' h] at h'
     exact h'
